theories/common/option.v
@@ -12,3 +12,10 @@ Proof.
   destruct o; done.
 Qed.
 
+#[global] Instance from_option_dec {A} (fn : A → Prop) `{∀ a, Decision (fn a)} default `{!Decision default} o : Decision (from_option fn default o) :=
+  match o with
+  | None =>
+      _
+  | Some _ =>
+      _
+  end.
